Added fixpoint operator to the object and lifted languages.

STLC_SuccNat/STLC_SuccNat.v
@@ -13,7 +13,9 @@ Inductive tm : Type :=
   | abs : string -> ty -> tm -> tm
 
   | const : nat -> tm
-  | succ : tm -> tm.
+  | succ : tm -> tm
+
+  | tm_fix : tm -> tm.
 
 Inductive value : tm -> Prop :=
   | v_abs : forall x T t, value (abs x T t)
@@ -29,6 +31,8 @@ Fixpoint subst (x : string) (s : tm) (t : tm) : tm :=
 
   | const _ => t
   | succ t1 => succ (subst x s t1)
+
+  | tm_fix t => tm_fix (subst x s t)
   end.
 
 (* Notation "[ x := s ] t" := (subst x s t) (at level 100).
@@ -36,21 +40,27 @@ Check [ "t" := const 1 ] (abs "t" Nat (succ (var "t"))). *)
 
 
 Inductive step : tm -> tm -> Prop :=
-  | ST_App1: forall t1 t1' t2,
-    step t1 t1' ->
-      step (app t1 t2) (app t1' t2)
-  | ST_App2: forall v t2 t2',
-    value v -> step t2 t2' ->
-      step (app v t2) (app v t2')
+  | ST_App1: forall t1 t2 t3,
+    step t1 t2 ->
+      step (app t1 t3) (app t2 t3)
+  | ST_App2: forall v t2 t3,
+    value v -> step t2 t3 ->
+      step (app v t2) (app v t3)
   | ST_AppAbs: forall x T t v,
     value v ->
       step (app (abs x T t) v) (subst x v t)
 
-  | ST_Succ: forall t1 t1',
-    step t1 t1' ->
-      step (succ t1) (succ t1')
+  | ST_Succ: forall t1 t2,
+    step t1 t2 ->
+      step (succ t1) (succ t2)
   | ST_SuccConst : forall (n : nat),
-    step (succ (const n)) (const (S n)).
+    step (succ (const n)) (const (S n))
+
+  | ST_Fix : forall t1 t2,
+    step t1 t2 ->
+      step (tm_fix t1) (tm_fix t2)
+  | ST_FixAbs : forall t1 T1 xf,
+    step (tm_fix (abs xf T1 t1)) (subst xf (tm_fix (abs xf T1 t1)) t1).
 
 Inductive multi {X : Type} (R : X -> X -> Prop) : X -> X -> Prop :=
   | multi_refl : forall (x : X), multi R x x
@@ -60,11 +70,11 @@ Inductive multi {X : Type} (R : X -> X -> Prop) : X -> X -> Prop :=
                     multi R x z.
 
 Definition normal_form {X : Type}
-              (R : X -> X -> Prop) (t : X) : Prop :=
-  ~(exists t', R t t').
+              (R : X -> X -> Prop) (t1 : X) : Prop :=
+  ~(exists t2, R t1 t2).
 
-Definition step_normal_form_of t t':=
-  (multi step t t' /\ normal_form step t').
+Definition step_normal_form_of t1 t2:=
+  (multi step t1 t2 /\ normal_form step t2).
 
 (*Typing*)
 Definition context := partial_map ty.
@@ -84,14 +94,18 @@ Inductive has_type : context -> tm -> ty -> Prop :=
   | T_Nat : forall Gamma (n : nat),
     has_type Gamma (const n) Nat
   | T_Succ : forall Gamma t,
-    has_type Gamma t Nat -> has_type Gamma (succ t) Nat.
+    has_type Gamma t Nat -> has_type Gamma (succ t) Nat
+
+  | T_Fix : forall Gamma t1 T1,
+    has_type Gamma t1 (Arrow T1 T1) ->
+    has_type Gamma (tm_fix t1) T1.
 
 
 (* Properties *)
-Lemma weakening : forall Gamma Gamma' t T,
-  includedin Gamma Gamma' ->
-  has_type Gamma t T ->
-  has_type Gamma' t T.
+Lemma weakening : forall Gamma1 Gamma2 t T,
+  includedin Gamma1 Gamma2 ->
+  has_type Gamma1 t T ->
+  has_type Gamma2 t T.
 Proof.
   intros Gamma Gamma' t T H Ht.
   generalize dependent Gamma'.
@@ -134,9 +148,9 @@ Ltac unfold_exists :=
       | [ H: exists _, _ |- _ ] => destruct H
   end.
 
-Theorem progress : forall t T,
-    has_type empty t T ->
-      value t \/ exists t', step t t'.
+Theorem progress : forall t1 T,
+    has_type empty t1 T ->
+      value t1 \/ exists t2, step t1 t2.
 Proof.
   intros t T Ht.
   remember empty as Gamma.
@@ -151,6 +165,12 @@ Proof.
     + eapply canonical_forms_nat in H as [n H]; subst; eauto.
       eexists. apply ST_SuccConst.
     + destruct H; eexists; eapply ST_Succ; eauto.
+  - right. destruct IHHt; auto.
+    + eapply canonical_forms_fun in Ht as [x [u Ht1]];
+      subst; auto; eexists.
+      apply ST_FixAbs.
+    + unfold_exists. exists (tm_fix x).
+      apply ST_Fix. auto.
 Qed.
 
 Lemma value_is_nf: forall t,
@@ -182,7 +202,7 @@ Theorem determinism : forall t1 t2 t3,
 Proof.
   intros t1 t2 t3 Ht.
   generalize dependent t3.
-  induction Ht; intros t3 Ht';
+  induction Ht; intros t4 Ht';
     inversion Ht'; subst; eauto;
     try value_no_step;
     try (f_equal; eauto);
@@ -209,39 +229,42 @@ Proof.
       rewrite n in H5. assumption.
 Qed.
 
-Theorem preservation: forall t t' T,
-  has_type empty t T ->
-  step t t' ->
-  has_type empty t' T.
+Theorem preservation: forall t1 t2 T,
+  has_type empty t1 T ->
+  step t1 t2 ->
+  has_type empty t2 T.
 Proof.
-  intros t t' T Ht;
-  generalize dependent t'.
+  intros t1 t2 T Ht;
+  generalize dependent t2.
   remember empty as Gamma.
-  induction Ht; intros t' H0;
+  induction Ht; intros t3 H0;
     inversion H0; subst;
       try (econstructor; eauto).
   apply (T_App _ _ _ _ _ Ht1) in Ht2.
   eapply substitution_preserves_typing;
     inversion Ht2; inversion H4; subst;
     eassumption.
+  inversion Ht; subst.
+  apply substitution_preserves_typing with T1;
+    try constructor; auto.
 Qed.
 
-Lemma preservation_multi: forall t t' T,
-  has_type empty t T ->
-  multi step t t' ->
-  has_type empty t' T.
+Lemma preservation_multi: forall t1 t2 T,
+  has_type empty t1 T ->
+  multi step t1 t2 ->
+  has_type empty t2 T.
 Proof.
-  intros t t' T Htype Hmulti.
+  intros t1 t2 T Htype Hmulti.
   induction Hmulti.
   - assumption.
   - apply (preservation _ _ _ Htype) in H.
     apply IHHmulti. apply H.
 Qed.
 
-Theorem normal_forms_unique: forall t1 t2 t2',
+Theorem normal_forms_unique: forall t1 t2 t3,
   step_normal_form_of t1 t2 ->
-  step_normal_form_of t1 t2' ->
-  t2 = t2'.
+  step_normal_form_of t1 t3 ->
+  t2 = t3.
 Proof.
   intros t1 t2 t2' P1 P2.
   destruct P1 as [P11 P12].
@@ -284,19 +307,19 @@ Proof.
     + exact H23.
 Qed.
 
-Lemma multistep_App2 : forall v t t',
-  value v -> (multi step t t') -> multi step (app v t) (app v t').
+Lemma multistep_App2 : forall v t1 t2,
+  value v -> (multi step t1 t2) -> multi step (app v t1) (app v t2).
 Proof.
-  intros v t t' V STM. induction STM.
+  intros v t1 t2 V STM. induction STM.
    apply multi_refl.
    eapply multi_step.
      apply ST_App2; eauto.  auto.
 Qed.
 
-Lemma multistep_succ : forall t t',
-  multi step t t' -> multi step (succ t) (succ t').
+Lemma multistep_succ : forall t1 t2,
+  multi step t1 t2 -> multi step (succ t1) (succ t2).
 Proof.
-  intros t t' STM. induction STM.
+  intros t1 t2 STM. induction STM.
    apply multi_refl.
    eapply multi_step.
      apply ST_Succ; eauto.  auto.
